Terms.v
@@ -1,0 +1,155 @@
+From Equations Require Import Equations.
+Require Import Coq.Setoids.Setoid.
+
+Require Import KA.Scope.
+Local Open Scope ka_scope.
+
+Section TermSyntax.
+  Context {A: Type}.
+
+  Inductive term :=
+  | zero: term
+  | one: term
+  | letter: A -> term
+  | plus: term -> term -> term
+  | times: term -> term -> term
+  | star: term -> term
+  .
+
+  Derive NoConfusion for term.
+End TermSyntax.
+
+Arguments term A : clear implicits.
+
+Notation "0" := zero : ka_scope.
+Notation "1" := one : ka_scope.
+Notation "$ a" :=
+  (letter a)
+  (at level 30)
+  : ka_scope
+.
+Notation "t1 + t2" :=
+  (plus t1 t2)
+  (at level 50, left associativity)
+  : ka_scope
+.
+Notation "t1 ;; t2" :=
+  (times t1 t2)
+  (at level 40, left associativity)
+  : ka_scope
+.
+Notation "t *" :=
+  (star t)
+  (at level 30)
+  : ka_scope
+.
+
+Section TermEquivalence.
+  Context {A: Type}.
+  Notation term := (term A).
+
+  Reserved Notation "t1 == t2" (at level 70).
+  Reserved Notation "t1 <= t2" (at level 70).
+
+  Inductive term_equiv: term -> term -> Prop :=
+  | ERefl: forall t, t == t
+  | ESym: forall t1 t2, t1 == t2 -> t2 == t1
+  | ETrans: forall t1 t2 t3, t1 == t2 -> t2 == t3 -> t1 == t3
+  | ECongPlus: forall t1 t2 t3 t4, t1 == t2 -> t3 == t4 -> t1 + t3 == t2 + t4
+  | ECongTimes: forall t1 t2 t3 t4, t1 == t2 -> t3 == t4 -> t1 ;; t3 == t2 ;; t4
+  | ECongStar: forall t1 t2, t1 == t2 -> t1 * == t2 *
+  | EPlusIdemp: forall t, t + t == t
+  | EPlusComm: forall t1 t2, t1 + t2 == t2 + t1
+  | EPlusAssoc: forall t1 t2 t3, t1 + (t2 + t3) == (t1 + t2) + t3
+  | EPlusUnit: forall t, t + 0 == t
+  | ETimesAssoc: forall t1 t2 t3, t1 ;; (t2 ;; t3) == (t1 ;; t2) ;; t3
+  | ETimesUnitRight: forall t, t ;; 1 == t
+  | ETimesUnitLeft: forall t, 1 ;; t == t
+  | ETimesZeroLeft: forall t, t ;; 0 == 0
+  | ETimesZeroRight: forall t, 0 ;; t == 0
+  | EDistributeLeft: forall t1 t2 t3, t1 ;; (t2 + t3) == t1 ;; t2 + t1 ;; t3
+  | EDistributeRight: forall t1 t2 t3, (t1 + t2) ;; t3 == t1 ;; t3 + t2 ;; t3
+  | EStarLeft: forall t, t* == t ;; t* + 1
+  | EFixLeft: forall t1 t2 t3, t2 ;; t1 + t3 <= t1 -> t2* ;; t3 <= t1
+  where "t1 == t2" := (term_equiv t1 t2) : ka_scope
+    and "t1 <= t2" := (t1 + t2 == t2) : ka_scope.
+
+  Global Add Relation term term_equiv
+    reflexivity proved by ERefl
+    symmetry proved by ESym
+    transitivity proved by ETrans
+    as equiv_eq
+  .
+
+  Global Add Morphism plus
+    with signature term_equiv ==> term_equiv ==> term_equiv
+    as plus_mor
+  .
+  Proof.
+    intros.
+    now apply ECongPlus.
+  Qed.
+
+  Global Add Morphism times
+    with signature term_equiv ==> term_equiv ==> term_equiv
+    as times_mor
+  .
+  Proof.
+    intros.
+    now apply ECongTimes.
+  Qed.
+
+  Global Add Morphism star
+    with signature term_equiv ==> term_equiv
+    as star_mor
+  .
+  Proof.
+    intros.
+    now apply ECongStar.
+  Qed.
+
+  Definition term_lequiv (t1 t2: term) := t1 <= t2.
+  (* Hint Unfold term_lequiv : core. *)
+
+  Lemma term_lequiv_refl (t: term):
+    t <= t
+  .
+  Proof.
+    now rewrite EPlusIdemp.
+  Qed.
+
+  Lemma term_lequiv_trans (t1 t2 t3: term):
+    t1 <= t2 -> t2 <= t3 -> t1 <= t3
+  .
+  Proof.
+    intros.
+    rewrite <- H0.
+    rewrite <- H.
+    repeat rewrite EPlusAssoc.
+    rewrite EPlusIdemp.
+    reflexivity.
+  Qed.
+
+  Lemma term_lequiv_zero (t: term):
+    0 <= t
+  .
+  Proof.
+    now rewrite EPlusComm, EPlusUnit.
+  Qed.
+
+  Global Add Relation term term_lequiv
+    reflexivity proved by term_lequiv_refl
+    transitivity proved by term_lequiv_trans
+    as term_lequiv_po
+  .
+
+  Global Instance term_equiv_implies_lequiv: subrelation term_equiv term_lequiv.
+  Proof.
+    unfold subrelation, term_lequiv; intros.
+    rewrite H.
+    now rewrite EPlusIdemp.
+  Qed.
+End TermEquivalence.
+
+Notation "t1 == t2" := (term_equiv t1 t2) (at level 70) : ka_scope.
+Notation "t1 <= t2" := (t1 + t2 == t2) (at level 70) : ka_scope.
