Vectors.v
@@ -1,0 +1,157 @@
+Require Import Coq.Setoids.Setoid.
+Require Import Coq.Program.Equality.
+
+Require Import KA.Terms.
+Require Import KA.Scope.
+Local Open Scope ka_scope.
+
+Section Vectors.
+  Variable (A: Type).
+  Notation term := (term A).
+
+  Inductive position: nat -> Type :=
+  | PHere:
+      forall {n: nat},
+      position (S n)
+  | PThere:
+      forall {n: nat}
+             (v: position n),
+      position (S n)
+  .
+
+  Definition vector (Q: Type) := Q -> term.
+
+  Definition matrix (Q: Type) := Q -> Q -> term.
+End Vectors.
+
+Section VectorOperations.
+  Context {A: Type}.
+  Notation term := (term A).
+  Notation vector := (vector A).
+  Notation matrix := (matrix A).
+
+  Definition vector_sum
+    {Q: Type}
+    (v1 v2: vector Q)
+    (q: Q)
+    : term
+  :=
+    (v1 q + v2 q)%ka
+  .
+
+  Definition vector_chomp
+    {n: nat}
+    (v: vector (position (S n)))
+    (p: position n)
+    : term
+  :=
+    v (PThere p)
+  .
+
+  Equations inner_product {n: nat} (v1 v2: vector (position n)): term := {
+    @inner_product 0 _ _ :=
+      zero;
+    @inner_product (S _) v1 v2 :=
+      v1 PHere ;; v2 PHere + inner_product (vector_chomp v1) (vector_chomp v2);
+  }.
+
+  Definition matrix_vector_product
+    {n: nat}
+    (m: matrix (position n))
+    (v: vector (position n))
+    (p: position n)
+  :=
+    inner_product (m p) v
+  .
+End VectorOperations.
+
+
+Notation "v1 <+> v2" := (vector_sum v1 v2) (at level 40) : ka_scope.
+Notation "# v" := (vector_chomp v) (at level 30) : ka_scope.
+Notation "v1 ** v2" := (inner_product v1 v2) (at level 40) : ka_scope.
+Notation "m <*> v" := (matrix_vector_product m v) (at level 40) : ka_scope.
+
+Section VectorEquiv.
+  Context {A: Type}.
+  Notation term := (term A).
+  Notation vector := (vector A).
+
+  Definition equiv_vec {Q: Type} (v1 v2: vector Q): Prop :=
+    forall (q: Q), v1 q == v2 q
+  .
+
+  Notation "v1 === v2" := (equiv_vec v1 v2) (at level 70).
+
+  Lemma equiv_vec_refl {Q: Type} (v: vector Q):
+    v === v
+  .
+  Proof.
+    now intro.
+  Qed.
+
+  Lemma equiv_vec_sym {Q: Type} (v1 v2: vector Q):
+    v1 === v2 -> v2 === v1
+  .
+  Proof.
+    intro; now intro.
+  Qed.
+
+  Lemma equiv_vec_trans {Q: Type} (v1 v2 v3: vector Q):
+    v1 === v2 -> v2 === v3 -> v1 === v3
+  .
+  Proof.
+    intros; intro.
+    now transitivity (v2 q).
+  Qed.
+
+  Global Add Parametric Relation (Q: Type): (vector Q) equiv_vec
+    reflexivity proved by equiv_vec_refl
+    symmetry proved by equiv_vec_sym
+    transitivity proved by equiv_vec_trans
+    as equiv_equiv_vec
+  .
+
+  Global Add Parametric Morphism (Q: Type): vector_sum
+    with signature (@equiv_vec Q) ==> equiv_vec ==> equiv_vec
+    as vector_sum_mor
+  .
+  Proof.
+    intros; intro.
+    unfold vector_sum.
+    now rewrite (H q), (H0 q).
+  Qed.
+
+  Global Add Parametric Morphism (n: nat): vector_chomp
+    with signature (@equiv_vec (position (S n))) ==> equiv_vec
+    as vector_comp_mor.
+  Proof.
+    intros.
+    intro.
+    unfold vector_chomp.
+    now rewrite (H (PThere q)).
+  Qed.
+
+  Global Add Parametric Morphism (n: nat): inner_product
+    with signature (@equiv_vec (position n)) ==> equiv_vec ==> term_equiv
+    as inner_product_mor
+  .
+  Proof.
+    intros.
+    dependent induction n.
+    - autorewrite with inner_product.
+      reflexivity.
+    - autorewrite with inner_product.
+      rewrite (H PHere), (H0 PHere).
+      apply ECongPlus; try reflexivity.
+      apply IHn.
+      + now rewrite H.
+      + now rewrite H0.
+  Qed.
+
+  Definition lequiv_vec {Q: Type} (v1 v2: vector Q): Prop :=
+    forall (q: Q), v1 q <= v2 q
+  .
+End VectorEquiv.
+
+Notation "v1 === v2" := (equiv_vec v1 v2) (at level 70) : ka_scope.
+Notation "v1 <== v2" := (lequiv_vec v1 v2) (at level 70) : ka_scope.
