Scope.v
@@ -1,0 +1,2 @@
+Declare Scope ka_scope.
+Delimit Scope ka_scope with ka.
